LambdaLetDollar.v
@@ -1,0 +1,427 @@
+Require Export Common.
+
+Inductive tm' {A} :=
+| tm_var' : A → tm'
+| tm_abs' : @tm' ^A → tm' (* λ  x. e *)
+| tm_s_0' : @tm' ^A → tm' (* S₀ f. e *)
+| tm_app' : tm' → tm' → tm' (* e   e *)
+| tm_dol' : tm' → tm' → tm' (* e $ e *)
+| tm_let' : tm' → @tm' ^A → tm' (* let x = e1 in e2 *)
+.
+Arguments tm' A : clear implicits.
+Global Hint Constructors tm' : core.
+
+Inductive val' {A} :=
+| val_abs' : @tm' ^A → val'
+.
+Arguments val' A : clear implicits.
+Global Hint Constructors val' : core.
+
+Definition val_to_tm' {A} (v : val' A) := 
+  match v with
+  | val_abs' e => tm_abs' e
+  end.
+
+Inductive non' {A} :=
+| non_s_0' : tm' ^A → non' (* S₀ f. e *)
+| non_app' : tm' A → tm'  A → non' (* e   e *)
+| non_dol' : tm' A → tm'  A → non' (* e $ e *)
+| non_let' : tm' A → tm' ^A → non' (* let x = e1 in e2 *)
+.
+
+Arguments non' A : clear implicits.
+Global Hint Constructors non' : core.
+
+Definition non_to_tm' {A} (p : non' A) := 
+  match p with
+  | non_s_0' e => tm_s_0' e
+  | non_app' e1 e2 => tm_app' e1 e2
+  | non_dol' e1 e2 => tm_dol' e1 e2
+  | non_let' e1 e2 => tm_let' e1 e2
+  end.
+
+Declare Custom Entry λ_let_dollar_scope.
+Notation "<{ e }>" := e (at level 1, e custom λ_let_dollar_scope at level 99).
+Notation "( x )" := x (in custom λ_let_dollar_scope, x at level 99).
+Notation "{ x }" := x (in custom λ_let_dollar_scope at level 0, x constr).
+Notation "x" := x (in custom λ_let_dollar_scope at level 0, x constr at level 0).
+Notation "'var' v" := (tm_var' v) (in custom λ_let_dollar_scope at level 1, left associativity).
+Notation "0" := <{ var None }> (in custom λ_let_dollar_scope at level 0).
+Notation "1" := <{ var {Some None} }> (in custom λ_let_dollar_scope at level 0).
+Notation "2" := <{ var {Some (Some None)} }> (in custom λ_let_dollar_scope at level 0).
+Notation "'λ' e" := (tm_abs' e)
+    (in custom λ_let_dollar_scope at level 90,
+      e custom λ_let_dollar_scope at level 99,
+      right associativity).
+Notation "'λv' e" := (val_abs' e)
+    (in custom λ_let_dollar_scope at level 90,
+      e custom λ_let_dollar_scope at level 99,
+      right associativity).
+Notation "'S₀' e" := (tm_s_0' e)
+    (in custom λ_let_dollar_scope at level 90,
+      e custom λ_let_dollar_scope at level 99,
+      right associativity).
+Notation "e1 e2" := (tm_app' e1 e2) (in custom λ_let_dollar_scope at level 10, left associativity).
+Notation "e1 '$' e2" := (tm_dol' e1 e2) (in custom λ_let_dollar_scope at level 80, right associativity).
+Notation "'let' e1 'in' e2" := (tm_let' e1 e2) (in custom λ_let_dollar_scope at level 70, right associativity).
+
+
+Fixpoint map' {A B : Type} (f : A -> B) (e : tm' A) : tm' B :=
+  match e with
+  | <{ var a }> => <{ var {f a} }>
+  | <{ λ  e' }> => <{ λ  {map' (option_map f) e'} }>
+  | <{ S₀ e' }> => <{ S₀ {map' (option_map f) e'} }>
+  | <{ e1   e2 }> => <{ {map' f e1}   {map' f e2} }>
+  | <{ e1 $ e2 }> => <{ {map' f e1} $ {map' f e2} }>
+  | <{ let e1 in e2 }> => tm_let' (map' f e1) (map' (option_map f) e2)
+  end.
+
+(* Lemma map_id_law : forall {V} (f : V -> V) e,
+  (forall x, f x = x) ->
+  f <$> e = e.
+Admitted.
+Lemma map_comp_law : forall A e B C (f:A->B) (g:B->C),
+  g <$> (f <$> e) = g ∘ f <$> e.
+Admitted. *)
+
+
+Fixpoint bind' {A B : Type} (f : A -> tm' B) (e : tm' A) : tm' B :=
+  match e with
+  | <{ var a }> => f a
+  | <{ e1   e2 }> => <{ {bind' f e1}   {bind' f e2} }>
+  | <{ e1 $ e2 }> => <{ {bind' f e1} $ {bind' f e2} }>
+  | <{ λ  e' }> => tm_abs' (bind' (fun a' => 
+      match a' with
+      | None   => tm_var' None
+      | Some a => map' Some (f a)
+      end) e')
+  | <{ S₀ e' }> => tm_s_0' (bind' (fun a' => 
+      match a' with
+      | None   => tm_var' None
+      | Some a => map' Some (f a)
+      end) e')
+  | <{ let e1 in e2 }> => tm_let' (bind' f e1) (bind' (fun a' => 
+      match a' with
+      | None   => tm_var' None
+      | Some a => map' Some (f a)
+      end) e2)
+  end.
+
+(* Lemma bind_is_map : forall A e B (f:A->B),
+  f <$> e = e >>= (fun v => tm_var (f v)).
+Admitted. *)
+
+(* Lemma bind_law : forall A e B C (f:A->tm' B) (g:B->tm' C),
+  e >>= f >>= g = e >>= (fun a => f a >>= g).
+Admitted. *)
+
+
+Definition var_subst' {V} e' (v:^V) :=
+  match v with
+  | None => e'
+  | Some v => <{ var v }>
+  end.
+
+Definition tm_subst0' {V} (e:tm' ^V) (v:val' V) :=
+  bind' (var_subst' (val_to_tm' v)) e.
+
+Notation "e [ 0 := v ]" := (tm_subst0' e v)
+  (in custom λ_let_dollar_scope at level 0,
+    e custom λ_let_dollar_scope,
+    v custom λ_let_dollar_scope at level 99).
+
+
+Definition tm_dec' (e : tm' ␀) : (val' ␀ + non' ␀) :=
+  match e with
+  | <{ var a }> => from_void a
+  | <{ λ  e' }> => inl (val_abs' e')
+  | <{ S₀ e' }> => inr (non_s_0' e')
+  | <{ e1   e2 }> => inr (non_app' e1 e2)
+  | <{ e1 $ e2 }> => inr (non_dol' e1 e2)
+  | <{ let e1 in e2 }> => inr (non_let' e1 e2)
+  end.
+
+
+Section Contexts.
+  Context {A : Type}.
+  Inductive J' :=
+  | J_fun' : tm'  A → J'  (* [] M *)
+  | J_arg' : val' A → J'  (* V [] *)
+  | J_dol' : tm'  A → J'  (* []$M *)
+  .
+  Inductive K' :=
+  | K_nil'  : K'
+  | K_cons' : J' → K' → K'
+  | K_let'  : K' → tm' ^A → K' (* let x = K in e *)
+  | K_del'  : val' A → K' → K' (* v $ K *) (* delimited *)  
+  .
+
+  Inductive T' :=
+  | T_nil'  : T'
+  | T_cons' : val' A → T' → T'  (* (v$) · T *)
+  .
+
+  Inductive redex' :=
+  | redex_beta'      : val' A → val' A → redex'
+  | redex_dollar'    : val' A → val' A → redex'
+  | redex_shift'     : val' A → tm' ^A → redex'  (* v $ S₀ f. e *)
+  | redex_dol_let'   : val' A → tm' ^A → tm' ^A → redex' (* v $ let x = S₀ f. e1 in e2 *)
+  | redex_let'       : J'     → non' A → redex'  (* J[p] *)
+  | redex_let_beta'  : val' A → tm' ^A → redex'  (* let x = v in e *)
+  | redex_let_assoc' : tm' ^A → tm' ^A → tm' ^A → redex' (* let x = (let y = S₀ f. e1 in e2) in e3 *)
+  .
+
+  Inductive dec' :=
+  | dec_value' : val' A → dec'
+  (* | dec_stuck' : K' → tm' ^A → dec' (* K[S₀ f. e] *) *)
+  | dec_stuck' : tm' ^A * option (tm' ^A) → dec' (* S₀ f. e1 | let x = S₀ f. e1 in e2 *)
+  (* | dec_stuck_s_0' : tm' ^A → dec' (* S₀ f. e1 *) *)
+  (* | dec_stuck_let' : tm' ^A → tm' ^A → dec' (* let x = S₀ f. e1 in e2 *) *)
+  | dec_redex' : K' → T' → redex' → dec' (* K[T[Redex]] *)
+  .
+
+  Definition dec_stuck_s_0' e := dec_stuck' (e, None).
+  Definition dec_stuck_let' e1 e2 := dec_stuck' (e1, (Some e2)).
+
+  Definition stuck_to_non' : tm' ^␀ * option (tm' ^␀) → non' ␀ := λ s,
+    match s with
+    | (e, None) => non_s_0' e
+    | (e1, Some e2) => non_let' <{ S₀ e1 }> e2
+    end.
+
+  Definition plugJ' j e' :=
+    match j with
+    | J_fun' e => <{ e' e }>
+    | J_arg' v => <{ {val_to_tm' v} e' }>
+    | J_dol' e => <{ e' $ e }>
+    end.
+  
+  Fixpoint plugK' k e :=
+    match k with
+    | K_nil' => e
+    (* | K_cons j k' => plugK' k' (plugJ' j e) *)
+    | K_cons' j k' => plugJ' j (plugK' k' e)
+    | K_let' k1 e2 => <{ let {plugK' k1 e} in e2 }>
+    | K_del' v1 k2 => <{ {val_to_tm' v1} $ {plugK' k2 e} }>
+    end.
+
+  Fixpoint plugT' trail e :=
+    match trail with
+    | T_nil' => e
+    (* | T_cons' v t => plugT' t <{ {val_to_tm' v} $ e }> *)
+    | T_cons' v t => <{ {val_to_tm' v} $ {plugT' t e} }>
+    end.
+
+  Definition redex_to_term' r := 
+    match r with
+    | redex_beta'   v1 v2 => <{ {val_to_tm' v1} {val_to_tm' v2} }>
+    | redex_dollar' v1 v2 => <{ {val_to_tm' v1} $ {val_to_tm' v2} }>
+    | redex_shift'  v  e  => <{ {val_to_tm' v } $  S₀ e }>
+    | redex_dol_let' v e1 e2 => <{ {val_to_tm' v } $ let S₀ e1 in e2 }>
+    | redex_let' j p  => plugJ' j (non_to_tm' p)
+    | redex_let_beta' v e => <{ let {val_to_tm' v} in e }>
+    | redex_let_assoc' e1 e2 e3 => <{ let (let S₀ e1 in e2) in e3 }>
+    end.
+
+End Contexts.
+Arguments J' A : clear implicits.
+Arguments K' A : clear implicits.
+Arguments T' A : clear implicits.
+Arguments redex' A : clear implicits.
+Arguments dec' A : clear implicits.
+
+
+Definition K_fun' {A} k e := @K_cons' A (J_fun' e) k.
+Definition K_arg' {A} v k := @K_cons' A (J_arg' v) k.
+Definition K_dol' {A} k e := @K_cons' A (J_dol' e) k.
+
+Fixpoint decompose' (e : tm' ␀) : dec' ␀ :=
+  match e with
+  | <{ var a }> => from_void a
+  | <{ λ  e' }> => dec_value' (val_abs' e')
+  | <{ S₀ e' }> => dec_stuck_s_0' e'
+  | <{ e1 e2 }> =>
+    match decompose' e1 with
+    | dec_stuck' s1    => dec_redex' (K_nil') T_nil' (redex_let' (J_fun' e2) (stuck_to_non' s1))
+    | dec_redex' k t r => dec_redex' (K_fun' k e2) t r
+    | dec_value' v1    => 
+      match decompose' e2 with
+      | dec_stuck' s2    => dec_redex' (K_nil') T_nil' (redex_let' (J_arg' v1) (stuck_to_non' s2))
+      | dec_redex' k t r => dec_redex' (K_arg' v1 k) t r
+      | dec_value' v2    => dec_redex' (K_nil') T_nil' (redex_beta' v1 v2)
+      end
+    end
+  | <{ e1 $ e2 }> =>
+    match decompose' e1 with
+    | dec_stuck' s1    => dec_redex' (K_nil') T_nil' (redex_let' (J_dol' e2) (stuck_to_non' s1))
+    | dec_redex' k t r => dec_redex' (K_dol' k e2) t r
+    | dec_value' v1    =>
+      match decompose' e2 with
+      | dec_stuck' (e2', None)       => dec_redex' K_nil' T_nil' (redex_shift' v1 e2')         (* v1 $ S₀ e2' *)
+      | dec_stuck' (e2_1, Some e2_2) => dec_redex' K_nil' T_nil' (redex_dol_let' v1 e2_1 e2_2) (* v1 $ let x = S₀ f. e2_1 in e2_2 *)
+      | dec_redex' k t r => dec_redex' (K_del' v1 k) t r  (* eval under the delimiter! *)
+      | dec_value' v2    => dec_redex' (K_nil') T_nil' (redex_dollar' v1 v2)
+      end
+    end
+  | <{ let e1 in e2 }> =>
+    match decompose' e1 with
+    | dec_stuck' (e1', None)       => dec_stuck_let' e1' e2 (* let x = S₀ f. e1' in e2 *)
+    | dec_stuck' (e1_1, Some e1_2) => dec_redex' K_nil' T_nil' (redex_let_assoc' e1_1 e1_2 e2) (* let x = (let y = S₀ f. e1_1 in e1_2) in e2 *)
+    | dec_redex' k t r => dec_redex' (K_let' k e2) t r
+    | dec_value' v1    => dec_redex' (K_nil') T_nil' (redex_let_beta' v1 e2) (* let x = v1 in e2 *)
+    end
+  end.
+
+(* Ltac inv_decompose_match H :=
+  match goal with
+  | H : (match decompose ?e with | dec_stuck _ _ | dec_redex _ _ _ | dec_value _ => _ end = _) |- _
+    => let d := fresh "d" in remember (decompose e) as d; inv d; inv_decompose_match H
+  | _ => try solve [inversion H; auto]; inj H
+  end. *)
+
+(* plug ∘ decompose = id *)
+(* Lemma decompose_value_inversion : ∀ e v,
+  decompose e = dec_value v → e = val_to_tm' v.
+Proof.
+  dependent inversion e; intros; cbn in *.
+  inversion v.
+  injection H; intros; subst; reflexivity.
+  inversion H.
+  remember (decompose t) as d; dependent induction d; try inversion H;
+  remember (decompose t0) as d0; dependent induction d0; try inversion H.
+  remember (decompose t) as d; dependent induction d; try inversion H;
+  remember (decompose t0) as d0; dependent induction d0; try inversion H.
+  Qed.
+
+Lemma decompose_stuck_inversion : ∀ e k e',
+  decompose e = dec_stuck k e' → e = plugK k <{ S₀ e' }>.
+Proof.
+  intros e k; generalize dependent e;
+  induction k; intros; inv e; cbn in *;
+  try solve [inversion a | inversion H | inj H; reflexivity];
+  inv_decompose_match H; cbn;
+  try rewrite (decompose_value_inversion e1 v); cbn; auto;
+  f_equal; apply IHk; auto.
+  Qed.
+
+Ltac inv_dec :=
+  match goal with
+  | H : dec_value ?v = decompose ?e |- _ => rewrite (decompose_value_inversion e v); cbn; auto
+  | H : dec_stuck ?k ?e' = decompose ?e |- _ => rewrite (decompose_stuck_inversion e k e'); cbn; auto
+  end.
+
+Lemma decompose_redex_inversion : ∀ e t k r,
+  decompose e = dec_redex k t r → e = plugK k (plugT t (redex_to_term r)).
+Proof.
+  dependent induction e; intros; cbn in *;
+  try solve [inversion a | inversion H | inv H];
+  inv_decompose_match H;
+  repeat inv_dec; cbn; f_equal; try solve [apply IHk; auto].
+  apply IHe2; auto.
+  apply IHe1; auto.
+  apply IHe2; auto.
+  apply IHe1; auto.
+  Qed.
+
+(* decompose ∘ plug = id *)
+Lemma decompose_plug_value : ∀ v,
+  decompose (val_to_tm' v) = dec_value v.
+Proof.
+  intros; destruct v; auto.
+  Qed.
+
+Lemma decompose_plug_stuck : ∀ k e, 
+  decompose (plugK k <{ S₀ e }>) = dec_stuck k e.
+Proof.
+  induction k; intros; cbn; auto.
+  inv j; cbn.
+  - rewrite IHk; auto.
+  - rewrite decompose_plug_value. rewrite IHk; auto.
+  - rewrite IHk; auto.
+  Qed.
+
+Lemma decompose_plug_redex : ∀ k t r,
+  decompose (plugK k (plugT t (redex_to_term r))) = dec_redex k t r.
+Proof with cbn; auto.
+  intros k t; generalize dependent k; induction t; intros...
+  - induction k...
+    + inv r; cbn; inv v; cbn; try solve [inv v0; auto].
+      rewrite decompose_plug_stuck; auto.
+    + inv j; try inv v; cbn; try solve [rewrite IHk; auto].
+  - induction k0...
+    + inv v... rewrite IHt...
+    + inv j; try inv v0; cbn; try solve [rewrite IHk0; auto].
+  Qed. *)
+
+
+Definition lift' {A : Type} (e : tm' A) : tm' ^A := map' Some e.
+
+Definition liftV' {A : Type} (v : val' A) : val' ^A :=
+  match v with
+  | val_abs' e => val_abs' (lift' e)
+  end.
+
+Definition liftJ' {A : Type} (j : J' A) : J' ^A := 
+  match j with
+  | J_fun' e => J_fun' (lift' e)
+  | J_arg' v => J_arg' (liftV' v)
+  | J_dol' e => J_dol' (lift' e)
+  end.
+
+Fixpoint liftK' {A : Type} (k : K' A) : K' ^A :=
+  match k with
+  | K_nil' => K_nil'
+  | K_cons' j k => K_cons' (liftJ' j) (liftK' k)
+  | K_let' k1 e2 => K_let' (liftK' k1) (lift' e2)
+  | K_del' v1 k2 => K_del' (liftV' v1) (liftK' k2)
+  end.
+
+(* Notation "↑ e" := (lift' e) (at level 15). *)
+
+Definition contract' (r : redex' ␀) : tm' ␀ :=
+  match r with
+  (* (λ x. e) v  ~>  e [x := v] *)
+  | redex_beta' (val_abs' e) v => <{ e [0 := v] }>
+
+  (* v1 $ v2  ~>  v1 v2 *)
+  | redex_dollar' v1 v2 => <{ {val_to_tm' v1} {val_to_tm' v2} }>
+
+  (* v $ S₀ f. e  ~>  e [f := λ x. v $ x] *)
+  | redex_shift' v e  => <{ e [0 := λv {lift' (val_to_tm' v)} $ 0] }>
+
+  (* v $ let x = S₀ f. e1 in e2  ~>  (λ x. v $ e2) $ S₀ f. e1 *)
+  | redex_dol_let' v e1 e2 => <{ (λ {lift' (val_to_tm' v)} $ e2) $ S₀ e1 }>
+
+  (* J[p]  ~>  let x = p in J[x] *)
+  | redex_let' j p => <{ let {non_to_tm' p} in {plugJ' (liftJ' j) <{ 0 }>} }>
+
+  (* let x = v in e  ~>  e [x := v] *)
+  | redex_let_beta' v e => <{ e [0 := v] }>
+
+  (* let x = (let y = S₀ f. e1 in e2) in e3  ~>  let y = S₀ f. e1 in let x = e2 in e3*)
+  | redex_let_assoc' e1 e2 e3 => <{ let S₀ e1 in let e2 in {lift' e3} }>
+  end.
+
+Definition step' e :=
+  match decompose' e with
+  | dec_redex' k t r => Some (plugK' k (plugT' t (contract' r)))
+  | _ => None
+  end.
+
+Fixpoint eval' i e :=
+  match i with
+  | 0 => e
+  | S j =>
+    match step' e with
+    | Some e' => eval' j e'
+    | None => e
+    end
+  end.
+
+Section Examples.
+  Definition _id : tm' ␀ := <{ λ 0 }>.
+  Definition _const : tm' ␀ := <{ λ λ 1 }>.
+
+  Compute (eval' 10 <{ _id $ _const $ S₀ 0 }>).
+  Compute (eval' 10 <{ _const $ _id $ S₀ 0 }>).
+End Examples.
